Vegas/Examples.lean
@@ -4,6 +4,7 @@ import Vegas.Examples.BattleOfTheSexes
 import Vegas.Examples.MontyHall
 import Vegas.Examples.SyntaxConstructors
 import Vegas.Examples.VegasLang
+import Vegas.Examples.NullableCommit
 import Vegas.Examples.BackendExamples
 import Vegas.Examples.SolutionConcepts
 import Vegas.Examples.StrategicSemantics
